Path.v
@@ -5,14 +5,53 @@ Module PathTheories  (O: UsualOrderedType)(S: FSetInterface.Sfun O)(G: Graph O S
   Module G := Graph.
 
   Import G.
+  
 
   Inductive path : graph -> vertex -> vertex -> Prop :=
   | p_start : forall g u v,
     contains_edge g u v = true -> path g u v
   | p_continue: forall g u v w,
-    contains_edge g u w = true ->
-    path g w v ->
+    path g u w ->
+    contains_edge g w v = true ->
     path g u v.
+
+  Inductive path' : graph -> vertex -> vertex -> Prop :=
+  | p_start' : forall g u v,
+    contains_edge g u v = true -> path' g u v
+  | p_continue': forall g u v w,
+    contains_edge g u w = true ->
+    path' g w v ->
+    path' g u v.
+
+  Lemma path_trans: forall g u v w,
+    path g u v ->
+    path g v w ->
+    path g u w.
+  Proof.
+    intros. induction H0.
+    - eapply p_continue. apply H. apply H0.
+    - eapply p_continue. apply IHpath. apply H. apply H1.
+  Qed.
+
+  Lemma path'_trans: forall g u v w,
+    path' g u v ->
+    path' g v w ->
+    path' g u w.
+  Proof.
+    intros. induction H. 
+    - eapply p_continue'. apply H. apply H0.
+    - eapply p_continue'. apply H. apply IHpath'. apply H0. 
+  Qed.
+
+  Lemma path_path': forall g v u,
+    path g u v <-> path' g u v.
+  Proof.
+    intros. split; intros H; induction H.
+    - apply p_start'. apply H.
+    - eapply path'_trans. apply IHpath. apply p_start'. apply H0.
+    - apply p_start. apply H.
+    - eapply path_trans. apply p_start. apply H. apply IHpath'.
+Qed.
 
   Fixpoint path_list (g: graph) (u v : vertex) (l: list vertex) : bool :=
     match l with
@@ -26,14 +65,34 @@ Module PathTheories  (O: UsualOrderedType)(S: FSetInterface.Sfun O)(G: Graph O S
   Lemma path_iff_list: forall g u v,
     path g u v <-> exists l, path_list g u v l = true.
   Proof.
-    intros. split; intros.
+    intros. rewrite path_path'. split; intros.
     - induction H.
       + exists nil. simpl. apply H.
-      + destruct IHpath. exists (w :: x). simpl. rewrite H. rewrite H1. reflexivity.
+      + destruct IHpath'. exists (w :: x). simpl. rewrite H. rewrite H1. reflexivity.
     - destruct H. generalize dependent u. induction x; intros. 
-      + simpl in H. apply p_start. apply H.
-      + simpl in H. rewrite andb_true_iff in H. destruct H.  eapply p_continue.  apply H.
+      + simpl in H. apply p_start'. apply H.
+      + simpl in H. rewrite andb_true_iff in H. destruct H.  eapply p_continue'.  apply H.
         apply IHx. apply H0.
+  Qed.
+
+  Inductive path_with: graph -> vertex -> vertex -> (vertex -> bool) -> Prop :=
+    |  pw_start : forall g u v f,
+      contains_edge g u v = true ->
+      f v = true ->
+      path_with g u v f
+    | pw_continue: forall g u v w f,
+      path_with g u w f ->
+      f v = true ->
+      contains_edge g w v = true ->
+      path_with g u v f.
+
+  Lemma path_with_implies_path: forall g u v f,
+    path_with g u v f ->
+    path g u v.
+  Proof.
+    intros. induction H.
+    - apply p_start. apply H.
+    - eapply p_continue. apply IHpath_with. apply H1.
   Qed.
 
   Definition cycle_exists (g: graph) := exists v, path g v v.
